HOL_To_IMP/HOL_Nat_To_IMP/Automation/HOL_Nat_To_IMP_Utils.thy
@@ -1,0 +1,13 @@
+\<^marker>\<open>creator "Kevin Kappelmann"\<close>
+theory HOL_Nat_To_IMP_Utils
+  imports
+    State_Update_Tracking
+    ML_Unification.Unify_Resolve_Tactics
+begin
+
+paragraph \<open>Summary\<close>
+text \<open>General ML utilities for the HOL to IMP refinement process.\<close>
+
+ML_file\<open>hol_nat_to_imp_util.ML\<close>
+
+end
