HOL_To_IMP/HOL_Nat_To_IMP/Automation/IMP_Terminates_With.thy
@@ -1,0 +1,202 @@
+\<^marker>\<open>creator "Kevin Kappelmann"\<close>
+theory IMP_Terminates_With
+  imports IMP.IMP_Tailcall
+begin
+
+definition "tailcall_to_IMP \<equiv> inline o compile"
+
+lemma tailcall_to_IMP_eq: "tailcall_to_IMP p = inline (compile p)"
+  unfolding tailcall_to_IMP_def by simp
+
+definition "terminates_with_pred_time_IMP p s s' P \<equiv> \<exists>t. (p, s) \<Rightarrow>\<^bsup>t\<^esup> s' \<and> P t"
+
+lemma terminates_with_pred_time_IMPI:
+  assumes "(p, s) \<Rightarrow>\<^bsup>t\<^esup> s'"
+  and "P t"
+  shows "terminates_with_pred_time_IMP p s s' P"
+  using assms unfolding terminates_with_pred_time_IMP_def by blast
+
+lemma terminates_with_pred_time_IMPE:
+  assumes "terminates_with_pred_time_IMP p s s' P"
+  obtains t where "(p, s) \<Rightarrow>\<^bsup>t\<^esup> s'" "P t"
+  using assms unfolding terminates_with_pred_time_IMP_def by blast
+
+definition "terminates_with_IMP p s s' \<equiv> terminates_with_pred_time_IMP p s s' (\<lambda>_. True)"
+
+lemma terminates_with_IMPI:
+  assumes "(p, s) \<Rightarrow>\<^bsup>t\<^esup> s'"
+  shows "terminates_with_IMP p s s'"
+  using assms terminates_with_pred_time_IMPI unfolding terminates_with_IMP_def by auto
+
+lemma terminates_with_IMPE:
+  assumes "terminates_with_IMP p s s'"
+  obtains t where "(p, s) \<Rightarrow>\<^bsup>t\<^esup> s'"
+  using assms terminates_with_pred_time_IMPE unfolding terminates_with_IMP_def by blast
+
+definition "terminates_with_res_pred_time_IMP p s r val P \<equiv>
+  \<exists>s'. terminates_with_pred_time_IMP p s s' P \<and> s' r = val"
+
+lemma terminates_with_res_pred_time_IMPI:
+  assumes "terminates_with_pred_time_IMP p s s' P"
+  and "s' r = val"
+  shows "terminates_with_res_pred_time_IMP p s r val P"
+  using assms unfolding terminates_with_res_pred_time_IMP_def by blast
+
+lemma terminates_with_res_pred_time_IMPE:
+  assumes "terminates_with_res_pred_time_IMP p s r val P"
+  obtains s' where "terminates_with_pred_time_IMP p s s' P" "s' r = val"
+  using assms unfolding terminates_with_res_pred_time_IMP_def by blast
+
+definition "terminates_with_res_IMP p s r val \<equiv>
+  terminates_with_res_pred_time_IMP p s r val (\<lambda>_. True)"
+
+lemma terminates_with_res_IMPI:
+  assumes "terminates_with_IMP p s s'"
+  and "s' r = val"
+  shows "terminates_with_res_IMP p s r val"
+  using assms unfolding terminates_with_res_IMP_def
+  by (intro terminates_with_res_pred_time_IMPI)
+  (simp only: flip: terminates_with_IMP_def)
+
+lemma terminates_with_res_IMPE:
+  assumes "terminates_with_res_IMP p s r val"
+  obtains s' where "terminates_with_IMP p s s'" "s' r = val"
+  using assms unfolding terminates_with_res_IMP_def
+  by (elim terminates_with_res_pred_time_IMPE)
+  (simp only: flip: terminates_with_IMP_def)
+
+definition "terminates_with_pred_time_IMP_Tailcall tp p s s' P \<equiv> \<exists>t. tp \<turnstile> (p, s) \<Rightarrow>\<^bsup>t\<^esup> s' \<and> P t"
+
+lemma terminates_with_pred_time_IMP_TailcallI:
+  assumes "tp \<turnstile> (p, s) \<Rightarrow>\<^bsup>t\<^esup> s'"
+  and "P t"
+  shows "terminates_with_pred_time_IMP_Tailcall tp p s s' P"
+  using assms unfolding terminates_with_pred_time_IMP_Tailcall_def by blast
+
+lemma terminates_with_pred_time_IMP_TailcallE:
+  assumes "terminates_with_pred_time_IMP_Tailcall tp p s s' P"
+  obtains t where "tp \<turnstile> (p, s) \<Rightarrow>\<^bsup>t\<^esup> s'" "P t"
+  using assms unfolding terminates_with_pred_time_IMP_Tailcall_def by blast
+
+definition "terminates_with_IMP_Tailcall tp p s s' \<equiv>
+  terminates_with_pred_time_IMP_Tailcall tp p s s' (\<lambda>_. True)"
+
+lemma terminates_with_IMP_TailcallI:
+  assumes "tp \<turnstile> (p, s) \<Rightarrow>\<^bsup>t\<^esup> s'"
+  shows "terminates_with_IMP_Tailcall tp p s s'"
+  using assms terminates_with_pred_time_IMP_TailcallI unfolding terminates_with_IMP_Tailcall_def by auto
+
+lemma terminates_with_IMP_TailcallE:
+  assumes "terminates_with_IMP_Tailcall tp p s s'"
+  obtains t where "tp \<turnstile> (p, s) \<Rightarrow>\<^bsup>t\<^esup> s'"
+  using assms terminates_with_pred_time_IMP_TailcallE unfolding terminates_with_IMP_Tailcall_def by blast
+
+definition "terminates_with_res_pred_time_IMP_Tailcall tp p s r val P \<equiv>
+  \<exists>s'. terminates_with_pred_time_IMP_Tailcall tp p s s' P \<and> s' r = val"
+
+lemma terminates_with_res_pred_time_IMP_TailcallI:
+  assumes "terminates_with_pred_time_IMP_Tailcall tp p s s' P"
+  and "s' r = val"
+  shows "terminates_with_res_pred_time_IMP_Tailcall tp p s r val P"
+  using assms unfolding terminates_with_res_pred_time_IMP_Tailcall_def by blast
+
+lemma terminates_with_res_pred_time_IMP_TailcallE:
+  assumes "terminates_with_res_pred_time_IMP_Tailcall tp p s r val P"
+  obtains s' where "terminates_with_pred_time_IMP_Tailcall tp p s s' P" "s' r = val"
+  using assms unfolding terminates_with_res_pred_time_IMP_Tailcall_def by blast
+
+definition "terminates_with_res_IMP_Tailcall tp p s r val \<equiv>
+  terminates_with_res_pred_time_IMP_Tailcall tp p s r val (\<lambda>_. True)"
+
+lemma terminates_with_res_IMP_TailcallI:
+  assumes "terminates_with_IMP_Tailcall tp p s s'"
+  and "s' r = val"
+  shows "terminates_with_res_IMP_Tailcall tp p s r val"
+  using assms unfolding terminates_with_res_IMP_Tailcall_def
+  by (intro terminates_with_res_pred_time_IMP_TailcallI)
+  (simp only: flip: terminates_with_IMP_Tailcall_def)
+
+lemma terminates_with_res_IMP_TailcallE:
+  assumes "terminates_with_res_IMP_Tailcall tp p s r val"
+  obtains s' where "terminates_with_IMP_Tailcall tp p s s'" "s' r = val"
+  using assms unfolding terminates_with_res_IMP_Tailcall_def
+  by (elim terminates_with_res_pred_time_IMP_TailcallE)
+  (simp only: flip: terminates_with_IMP_Tailcall_def)
+
+context
+  notes
+    terminates_with_IMPE[elim] terminates_with_res_IMPE[elim]
+    terminates_with_IMP_TailcallE[elim] terminates_with_res_IMP_TailcallE[elim]
+    terminates_with_res_IMPI[intro] terminates_with_IMPI[intro]
+    terminates_with_res_IMP_TailcallI[intro] terminates_with_IMP_TailcallI[intro]
+begin
+
+lemma terminates_with_res_IMP_if_terminates_with_res_IMP_TailcallI:
+  assumes "invar p"
+  and "r \<in> set (vars p)"
+  and "terminates_with_res_IMP_Tailcall p p s r val"
+  shows "terminates_with_res_IMP (tailcall_to_IMP p) s r val"
+  using assms by (elim terminates_with_res_IMP_TailcallE terminates_with_IMP_TailcallE
+    compile_sound inline_sound[where ?s=s and ?s'=s for s])
+  (force simp: set_vars_compile tailcall_to_IMP_eq)+
+
+lemma terminates_with_tSeqI:
+  assumes "terminates_with_IMP_Tailcall p p1 s s'"
+  and "terminates_with_IMP_Tailcall p p2 s' s''"
+  shows "terminates_with_IMP_Tailcall p (tSeq p1 p2) s s''"
+  using assms by blast
+
+lemma terminates_with_tAssignI:
+  assumes "s' = s(k := aval aexp s)"
+  shows "terminates_with_IMP_Tailcall p (tAssign k aexp) s s'"
+  using assms by blast
+
+lemma terminates_with_tIfI:
+  assumes "s vb \<noteq> 0 \<Longrightarrow> terminates_with_IMP_Tailcall p p1 s s'"
+  and "s vb = 0 \<Longrightarrow> terminates_with_IMP_Tailcall p p2 s s'"
+  shows "terminates_with_IMP_Tailcall p (tIf vb p1 p2) s s'"
+  using assms by (cases "s vb = 0") blast+
+
+lemma terminates_with_tCallI:
+  assumes "terminates_with_res_IMP p s r val"
+  and "s' = s(r := val)"
+  shows "terminates_with_IMP_Tailcall tp (tCall p r) s s'"
+  using assms by blast
+
+lemma terminates_with_tTailI:
+  assumes "terminates_with_IMP_Tailcall p p s s'"
+  shows "terminates_with_IMP_Tailcall p tTAIL s s'"
+  using assms by blast+
+
+lemma terminates_with_res_tSeqI:
+  assumes "terminates_with_IMP_Tailcall p p1 s s'"
+  and "terminates_with_res_IMP_Tailcall p p2 s' r val"
+  shows "terminates_with_res_IMP_Tailcall p (tSeq p1 p2) s r val"
+  using assms by blast
+
+lemma terminates_with_res_tAssignI:
+  assumes "s' = s(k := aval aexp s)"
+  and "s' r = val"
+  shows "terminates_with_res_IMP_Tailcall p (tAssign k aexp) s r val"
+  using assms by blast
+
+lemma terminates_with_res_tIfI:
+  assumes "s vb \<noteq> 0 \<Longrightarrow> terminates_with_res_IMP_Tailcall p p1 s r val"
+  and "s vb = 0 \<Longrightarrow> terminates_with_res_IMP_Tailcall p p2 s r val"
+  shows "terminates_with_res_IMP_Tailcall p (tIf vb p1 p2) s r val"
+  using assms by (cases "s vb = 0") blast+
+
+lemma terminates_with_res_tCallI:
+  assumes "terminates_with_res_IMP p s r val"
+  and "(s(r := val)) r' = val'"
+  shows "terminates_with_res_IMP_Tailcall tp (tCall p r) s r' val'"
+  using assms by blast
+
+lemma terminates_with_res_tTailI:
+  assumes "terminates_with_res_IMP_Tailcall p p s r val"
+  shows "terminates_with_res_IMP_Tailcall p tTAIL s r val"
+  using assms by blast+
+
+end
+
+end
