HOL_To_IMP/HOL_Nat_To_IMP/States/States_Base.thy
@@ -1,0 +1,43 @@
+\<^marker>\<open>creator "Kevin Kappelmann"\<close>
+theory States_Base
+  imports
+    (* Trie.Trie *)
+    Main
+begin
+
+paragraph \<open>Summary\<close>
+text \<open>States are abstractions of functions with updates.\<close>
+
+(*an alternative using tries, which turned out to be too slow because the construction of the trie
+cannot be evaluated by normalisation as it is*)
+(* datatype ('k, 'v) state = State "('k, 'v) trie \<times> ('k list \<Rightarrow> 'v)"
+
+definition "interp_state s k \<equiv> case_state (\<lambda>(t, s). case lookup_trie t k of None \<Rightarrow> s k | Some v \<Rightarrow> v) s"
+
+definition "state s \<equiv> State (empty_trie, s)"
+
+lemma interp_state_state_eq: "interp_state (state s) = s"
+  unfolding interp_state_def state_def by simp
+
+definition "update_state k v \<equiv> case_state (\<lambda>(t, s). State (update_trie k v t, s))"
+
+lemma interp_update_state_eq: "interp_state (update_state k v st) = (interp_state st)(k := v)"
+  unfolding update_state_def interp_state_def
+  by (cases st) (auto split: prod.splits option.splits simp: lookup_update) *)
+
+datatype ('k, 'v) state = State "('k list \<Rightarrow> 'v)"
+
+definition "interp_state s k \<equiv> case_state (\<lambda>s. s k) s"
+
+definition "state s \<equiv> State s"
+
+lemma interp_state_state_eq: "interp_state (state s) = s"
+  unfolding interp_state_def state_def by simp
+
+definition "update_state k v \<equiv> case_state (\<lambda>s. State (s(k := v)))"
+
+lemma interp_update_state_eq: "interp_state (update_state k v st) = (interp_state st)(k := v)"
+  unfolding update_state_def interp_state_def
+  by (cases st) (auto split: prod.splits option.splits)
+
+end
