HOL_To_IMP/HOL_To_HOL_Nat/HOL_To_HOL_Nat_Tests.thy
@@ -1,0 +1,58 @@
+\<^marker>\<open>creator "Jay Neubrand"\<close>
+\<^marker>\<open>creator "Andreas Vollert"\<close>
+\<^marker>\<open>contributor "Kevin Kappelmann"\<close>
+theory HOL_To_HOL_Nat_Tests
+  imports
+    HOL_To_HOL_Nat_Basics
+begin
+
+context
+  includes lifting_syntax
+  notes transport_eq_id.partial_equivalence_rel_equivalenceI[per_intro del]
+  and transport_eq_restrict_id.partial_equivalence_rel_equivalence[per_intro del]
+begin
+
+fun elemof :: "'a \<Rightarrow> 'a list \<Rightarrow> bool" where
+  "elemof _ [] = False"
+| "elemof y (x#xs) = (if (y = x) then True else elemof y xs)"
+
+case_of_simps elemof_eq_case : elemof.simps
+function_compile_nat elemof_eq_case
+print_theorems
+
+lemma If_eq_case: "If = (\<lambda>b x y. (case b of True \<Rightarrow> x | False \<Rightarrow> y))"
+  by (intro ext) simp
+
+function_compile_nat If_eq_case
+print_theorems
+
+fun takeWhile :: "('a \<Rightarrow> bool) \<Rightarrow> 'a list \<Rightarrow> 'a list" where
+  "takeWhile P [] = []" |
+  "takeWhile P (x # xs) = (if P x then x # takeWhile P xs else [])"
+
+case_of_simps takeWhile_eq_case : takeWhile.simps
+function_compile_nat takeWhile_eq_case
+print_theorems
+
+fun head :: "bool list \<Rightarrow> bool" where
+  "head [] = undefined" |
+  "head (x # _) = x"
+
+lemma Rel_nat_undefined [Rel_nat]:
+  "Rel_nat (natify (undefined :: 'a :: compile_nat)) (undefined :: 'a)"
+  by (rule Rel_nat_natify_self)
+
+case_of_simps head_eq_case : head.simps
+function_compile_nat head_eq_case
+
+fun plus :: "nat \<Rightarrow> nat \<Rightarrow> nat" where
+  "plus m 0 = m" |
+  "plus m (Suc n) = plus (Suc (plus m n)) 0"
+
+case_of_simps plus_eq_case : plus.simps
+function_compile_nat plus_eq_case
+print_theorems
+
+end
+
+end
