HOL_To_IMP/Refinements/HOL_To_IMP_Arithmetics.thy
@@ -1,0 +1,117 @@
+\<^marker>\<open>creator "Kevin Kappelmann"\<close>
+theory HOL_To_IMP_Arithmetics
+  imports
+    HOL_To_IMP_Primitives
+    "HOL-Library.Discrete_Functions"
+begin
+
+paragraph \<open>Power\<close>
+
+context HOL_To_HOL_Nat
+begin
+
+fun power_acc_nat :: "nat \<Rightarrow> nat \<Rightarrow> nat \<Rightarrow> nat" where
+"power_acc_nat x 0 acc = acc" |
+"power_acc_nat x (Suc n) acc = power_acc_nat x n (x * acc)"
+declare power_acc_nat.simps[simp del]
+
+lemma power_acc_nat_eq_power_mul: "power_acc_nat x y z = x^y * z"
+  by (induction x y z arbitrary: z rule: power_acc_nat.induct)
+  (auto simp: power_acc_nat.simps)
+
+case_of_simps power_acc_nat_eq : power_acc_nat.simps
+function_compile_nat power_acc_nat_eq
+
+lemma power_eq_power_acc_nat_one: "x^y = power_acc_nat x y 1"
+  using power_acc_nat_eq_power_mul by simp
+
+function_compile_nat power_eq_power_acc_nat_one
+
+end
+
+context HOL_Nat_To_IMP
+begin
+
+lemmas power_acc_nat_nat_eq = HTHN.power_acc_nat_nat_eq_unfolded[unfolded case_nat_eq_if]
+compile_nat power_acc_nat_nat_eq basename power_acc
+HOL_To_IMP_correct HTHN.power_acc_nat_nat by cook
+
+compile_nat HTHN.power_nat_eq_unfolded basename power
+HOL_To_IMP_correct HTHN.power_nat by cook
+
+end
+
+context HOL_To_HOL_Nat
+begin
+
+(*takes lower and upper bound for root*)
+function sqrt_aux_nat :: "nat \<Rightarrow> nat \<Rightarrow> nat \<Rightarrow> nat" where
+  "sqrt_aux_nat x L R = (if Suc L < R
+    then
+      let M = (L + R) div 2
+      in
+        if M\<^sup>2 \<le> x
+        then sqrt_aux_nat x M R
+        else sqrt_aux_nat x L M
+    else L)"
+  by auto
+termination by (relation "Wellfounded.measure (\<lambda>(_, L, R). R - L)") auto
+declare sqrt_aux_nat.simps[simp del]
+
+lemma square_sqrt_aux_nat_le:
+  assumes "L\<^sup>2 \<le> x" "x < R\<^sup>2"
+  shows "(sqrt_aux_nat x L R)\<^sup>2 \<le> x"
+  using assms
+  by (induction x L R rule: sqrt_aux_nat.induct)
+  (auto simp: sqrt_aux_nat.simps Let_def)
+
+lemma lt_square_Suc_sqrt_aux_nat:
+  assumes "L\<^sup>2 \<le> x" "x < R\<^sup>2"
+  shows "x < (Suc (sqrt_aux_nat x L R))\<^sup>2"
+  using assms
+  by (induction x L R rule: sqrt_aux_nat.induct)
+  (use order_less_le_trans in \<open>force simp: sqrt_aux_nat.simps Let_def\<close>)
+
+function_compile_nat sqrt_aux_nat.simps
+
+definition sqrt_nat :: "nat \<Rightarrow> nat" where
+  "sqrt_nat x = sqrt_aux_nat x 0 (Suc x)"
+
+lemma square_sqrt_nat_le: "(sqrt_nat x)\<^sup>2 \<le> x"
+  using square_sqrt_aux_nat_le unfolding sqrt_nat_def by (simp add: power2_eq_square)
+
+lemma lt_square_Suc_sqrt_nat: "x < (Suc (sqrt_nat x))\<^sup>2"
+  using lt_square_Suc_sqrt_aux_nat unfolding sqrt_nat_def by (simp add: power2_eq_square)
+
+corollary sqrt_nat_eq: "sqrt_nat y = floor_sqrt y"
+  using square_sqrt_nat_le lt_square_Suc_sqrt_nat
+  by (intro floor_sqrt_unique[symmetric]) auto
+
+corollary floor_sqrt_eq_sqrt_aux_nat: "floor_sqrt x = sqrt_aux_nat x 0 (Suc x)"
+  using sqrt_nat_eq sqrt_nat_def by simp
+
+function_compile_nat sqrt_nat_def
+
+end
+
+context HOL_Nat_To_IMP
+begin
+
+compile_nat HTHN.sqrt_aux_nat_nat_eq_unfolded
+HOL_To_IMP_correct HTHN.sqrt_aux_nat_nat by cook
+  (*Example step-by-step tactic invocation for debugging purposes.*)
+  (* apply (tactic \<open>HM.correct_if_IMP_tailcall_correct_tac HT.get_IMP_def @{context} 1\<close>)
+  apply (tactic \<open>HT.setup_induction_tac HT.get_fun_inducts @{context} 1\<close>)
+  apply (tactic \<open>HT.start_case_tac HT.get_IMP_def @{context} 1\<close>)
+  apply (tactic \<open>HT.run_tac HT.get_imp_correct @{context} 1\<close>)
+  apply (tactic \<open>SOLVED' (HT.finish_tac HB.get_HOL_eqs @{context}) 1\<close>)
+  apply (tactic \<open>SOLVED' (HT.finish_tac HB.get_HOL_eqs @{context}) 1\<close>)
+  apply (tactic \<open>SOLVED' (HT.finish_tac HB.get_HOL_eqs @{context}) 1\<close>)
+  oops *)
+
+compile_nat HTHN.sqrt_nat_nat_eq_unfolded
+HOL_To_IMP_correct HTHN.sqrt_nat_nat by cook
+
+end
+
+end
