HOL_To_IMP/Refinements/HOL_To_IMP_Pairs.thy
@@ -1,0 +1,40 @@
+\<^marker>\<open>creator "Kevin Kappelmann"\<close>
+theory HOL_To_IMP_Pairs
+  imports
+    HOL_To_IMP_Arithmetics
+begin
+
+context HOL_To_HOL_Nat
+begin
+
+function_compile_nat fst_def
+function_compile_nat snd_def
+
+definition "rpair y x \<equiv> (x, y)"
+
+function_compile_nat rpair_def
+
+end
+
+context HOL_Nat_To_IMP
+begin
+
+declare Rel_nat_selector_prod[Rel_nat]
+
+compile_nat Pair_nat_def
+HOL_To_IMP_correct Pair_nat by cook
+
+lemmas fst_nat_eq = HTHN.fst_nat_eq_unfolded[unfolded case_prod_nat_def]
+compile_nat fst_nat_eq
+HOL_To_IMP_correct HOL_To_HOL_Nat.fst_nat by cook
+
+lemmas snd_nat_eq = HTHN.snd_nat_eq_unfolded[unfolded case_prod_nat_def]
+compile_nat snd_nat_eq
+HOL_To_IMP_correct HOL_To_HOL_Nat.snd_nat by cook
+
+compile_nat HTHN.rpair_nat_eq_unfolded
+HOL_To_IMP_correct HOL_To_HOL_Nat.rpair_nat by cook
+
+end
+
+end
