IMP-/IMP_To_IMP-/Binary_Operations.thy
@@ -1,0 +1,841 @@
+\<^marker>\<open>creator Florian Keßler\<close>
+\<^marker>\<open>creator Fabian Huch\<close>
+
+section "Binary Operations in IMP-"
+
+theory Binary_Operations
+  imports
+    IMP_To_IMP_Minus_State_Translations
+    "IMP.Com"
+    "IMP-.IMP_Minus_Subprograms" 
+begin
+
+text \<open> We give programs in IMP- that work on states translated from IMP to IMP- and simulate
+       the arithmetic expressions of IMP. They work by first loading the operands into some special
+       operand registers, and then performing standard binary addition / subtraction. \<close>
+
+type_synonym IMP_com = Com.com
+type_synonym IMP_Minus_com = "IMP_Minus_Com.com"
+
+unbundle no Com.com_syntax
+
+fun com_list_to_seq:: "IMP_Minus_com list \<Rightarrow> IMP_Minus_com" where
+"com_list_to_seq [] = SKIP" |
+"com_list_to_seq (c # cs) = c ;; (com_list_to_seq cs)"
+
+lemma t_small_step_fun_com_list_to_seq_terminates: "t1 + t2 < t
+  \<Longrightarrow> t_small_step_fun t1 (com_list_to_seq as, s1) = (SKIP, s3)
+  \<Longrightarrow> t_small_step_fun t2 (com_list_to_seq bs, s3) = (SKIP, s2)
+  \<Longrightarrow> t_small_step_fun t (com_list_to_seq (as @ bs), s1) = (SKIP, s2)"
+proof(induction as arbitrary: s1 t1 t)
+  case Nil
+  then show ?case using t_small_step_fun_increase_time
+    by (metis Pair_inject append_self_conv2 com_list_to_seq.simps le_add2
+        less_imp_le_nat t_small_step_fun_SKIP)
+next
+  case (Cons a as)
+  then obtain ta sa where ta_def: "ta < t1 \<and> t_small_step_fun ta (a, s1) = (SKIP, sa)
+    \<and> t_small_step_fun (t1 - (ta + 1)) (com_list_to_seq as, sa) = (SKIP, s3)"
+    by (auto simp: seq_terminates_iff)
+  hence "t_small_step_fun (t - (ta + 1)) (com_list_to_seq (as @ bs), sa) = (SKIP, s2)"
+    apply -
+    apply(rule Cons(1))
+    using Cons by(auto)
+  thus ?case using ta_def Cons seq_terminates_iff by fastforce
+qed
+
+thm_oracles t_small_step_fun_com_list_to_seq_terminates
+
+declare seq_terminates_when'[intro]
+lemma tsmall_seq [intro]: "
+  t_small_step_fun t1 (c1, s1) = (SKIP, s2) \<Longrightarrow>
+  t_small_step_fun t2 (c2, s2) = (SKIP, s3) \<Longrightarrow> 
+t_small_step_fun (t1+t2+1) (c1;;c2, s1) = (SKIP, s3)"
+  by (meson less_add_one seq_terminates_when')
+
+lemma com_list_to_seq_of_length_one_terminates_iff:
+  "t_small_step_fun t (com_list_to_seq [c], s1) = (SKIP, s2) \<longleftrightarrow>
+  (t > 0 \<and> t_small_step_fun (t - 1) (c, s1) = (SKIP, s2))"
+  apply(auto simp: seq_terminates_iff)
+  using t_small_step_fun_increase_time apply (metis One_nat_def diff_Suc_1 le_add1 less_imp_Suc_add)
+  using diff_Suc_less by blast
+
+lemma com_list_to_seq_variables: "set (enumerate_variables (com_list_to_seq cs))
+  = { v | v c. c \<in> set cs \<and> v \<in> set (enumerate_variables c)}"
+  apply(induction cs)
+  by(auto simp: set_enumerate_variables_seq)
+
+text \<open>Computing enumerate_variables is too slow for the _anything_, this does it quickly:\<close>
+fun lvarS :: "com \<Rightarrow> vname set" where
+  "lvarS (Assign v _) = {v}" |
+  "lvarS (c1;;c2) = lvarS c1 \<union> lvarS c2" |
+  "lvarS (If v c1 c2) = {v} \<union> lvarS c1 \<union>lvarS c2" |
+  "lvarS (While v c) = {v} \<union> lvarS c" |
+  "lvarS _ = {}"
+
+lemma larvs_set_enum: "lvarS c = set (enumerate_variables c)"
+  apply (induction c) 
+  apply simp_all
+  using set_enumerate_variables_seq apply presburger
+  using set_enumerate_variables_if apply auto[1]
+  using set_enumerate_variables_while by auto
+
+fun binary_assign_constant_bits:: "nat \<Rightarrow> vname \<Rightarrow> nat \<Rightarrow> IMP_Minus_com" where
+"binary_assign_constant_bits 0 v x = SKIP" |
+"binary_assign_constant_bits (Suc n) v x = (var_bit_to_var (v, (Suc n))) ::= nth_bit x n ;;
+  binary_assign_constant_bits n v x"
+
+lemma result_of_binary_assign_constant_bits: "t_small_step_fun (3 * n)
+  (binary_assign_constant_bits n v x, s)
+  = (SKIP, \<lambda>w. (case var_to_var_bit w of
+      Some (w', Suc m) \<Rightarrow> (if w' = v \<and> m < n then Some (nth_bit x m) else s w) |
+      _ \<Rightarrow> s w))"
+proof(induction n arbitrary: s)
+  case (Suc n)
+  thus ?case
+    apply auto
+    apply(rule seq_terminates_when[where ?t1.0=1 and ?t2.0="3*n" and
+          ?s3.0="s(var_bit_to_var (v, Suc n) \<mapsto> nth_bit x n)"])
+    by(auto simp: fun_eq_iff var_to_var_bit_eq_Some_iff  split: option.splits nat.splits)
+qed (auto simp: fun_eq_iff split: option.splits nat.splits)
+
+lemma binary_assign_constant_bits_variables[simp]: 
+  "set (enumerate_variables (binary_assign_constant_bits n v x)) = { var_bit_to_var (v, Suc i) | i. i < n }"
+  apply(induction n)
+  by(auto simp: set_enumerate_variables_seq)
+
+definition binary_assign_zero :: "nat \<Rightarrow> vname \<Rightarrow> nat \<Rightarrow> IMP_Minus_com" where
+"binary_assign_zero n v x = (var_bit_to_var (v, 0)) ::= zero_bit x n"
+
+lemma result_of_binary_assign_zero: "t_small_step_fun 1
+  (binary_assign_zero n v x, s) 
+  = (SKIP, \<lambda>w. (case var_to_var_bit w of
+      Some (w',m) \<Rightarrow> (if w' = v \<and> m = 0 then Some (zero_bit x n) else s w ) | _ \<Rightarrow> s w))"
+  unfolding binary_assign_zero_def
+  by (auto simp: numeral_eq_Suc var_to_var_bit_eq_Some_iff fun_eq_iff split: option.splits)
+
+lemma binary_assign_zero_vars: "enumerate_variables (binary_assign_zero n v x) = [var_bit_to_var (v,0)]"
+  unfolding binary_assign_zero_def by simp
+
+definition "binary_assign_constant n v x = binary_assign_zero n v x;; binary_assign_constant_bits n v x"
+declare [[names_short]]
+
+lemma binary_assign_constant_ne_Skip[simp]: "binary_assign_constant n v x \<noteq> SKIP"
+  unfolding binary_assign_constant_def by auto
+
+lemma result_of_binary_assign_constant:
+  "t_small_step_fun (3 * n + 2)
+  (binary_assign_constant n v x, s)
+  = (SKIP, \<lambda>w. (case var_to_var_bit w of
+      Some (w', m) \<Rightarrow> if w' = v then 
+        (case m of 0 \<Rightarrow> Some (zero_bit x n)
+                 | Suc m \<Rightarrow> if m < n then Some (nth_bit x m) else s w)
+        else s w |
+      _ \<Rightarrow> s w))"
+  unfolding binary_assign_constant_def
+  apply (rule seq_terminates_when[of 1 "3*n"])
+  apply simp
+   apply (rule result_of_binary_assign_zero)
+  apply (subst result_of_binary_assign_constant_bits[of n v x])
+  by (auto simp add: fun_eq_iff split: option.splits if_splits nat.splits)
+
+lemma binary_assign_constant_variables[simp]: "set (enumerate_variables (binary_assign_constant n v x))
+  = {var_bit_to_var (v, Suc i) | i. i < n} \<union> { var_bit_to_var (v, 0)}"
+  apply (subst larvs_set_enum[symmetric]) 
+  unfolding binary_assign_constant_def binary_assign_zero_def
+  apply auto
+   apply (auto simp add: larvs_set_enum)
+  done
+
+lemma result_of_binary_assign_constant_on_translated_state_aux:
+  assumes "n > 0"
+  shows "t_small_step_fun (3 * n+2) (binary_assign_constant n v x,
+    IMP_State_To_IMP_Minus s n)
+    = (SKIP, IMP_State_To_IMP_Minus (s(v := x)) n)"
+  unfolding binary_assign_constant_def
+  apply (rule seq_terminates_when[of 1 "3*n"])
+  apply simp
+   apply (rule result_of_binary_assign_zero)
+  unfolding IMP_State_To_IMP_Minus_def
+  using result_of_binary_assign_constant_bits[of n v x] 
+  by (simp add: fun_eq_iff
+  IMP_State_To_IMP_Minus_with_operands_a_b_def split: option.splits nat.splits)
+
+lemma result_of_binary_assign_constant_on_translated_state:
+  assumes "n > 0"
+  shows "t_small_step_fun (50 * (n + 2)) (binary_assign_constant n v x,
+    IMP_State_To_IMP_Minus s n)
+    = (SKIP, IMP_State_To_IMP_Minus (s(v := x)) n)"
+  apply(rule t_small_step_fun_increase_time[where ?t="3*n+2"])
+  apply simp
+  apply(subst result_of_binary_assign_constant_on_translated_state_aux)
+  using assms by auto
+
+fun copy_var_to_operand:: "nat \<Rightarrow> char \<Rightarrow> vname \<Rightarrow> IMP_Minus_com" where
+"copy_var_to_operand 0 op v = SKIP" |
+"copy_var_to_operand (Suc i) op v =
+   (IF var_bit_to_var (v, Suc i) \<noteq>0 THEN
+   (operand_bit_to_var (op, i)) ::= One
+    ELSE
+    (operand_bit_to_var (op, i)) ::= Zero) ;;
+    copy_var_to_operand i op v"
+
+lemma copy_var_to_operand_result:
+  "t_small_step_fun (4 * n) (copy_var_to_operand n op v, s)
+  = (SKIP, \<lambda>w. (case var_to_operand_bit w of
+    Some (op', i) \<Rightarrow> (if op' = op \<and> i < n
+  then (case s (var_bit_to_var (v, Suc i)) of Some x \<Rightarrow> Some x | None \<Rightarrow> Some One)
+  else s w) |
+    _ \<Rightarrow> s w))"
+proof(induction n arbitrary: s)
+  case 0
+  then show ?case by (auto simp: fun_eq_iff split: option.splits)
+next
+  case (Suc n)
+  let ?s' = "s(operand_bit_to_var (op, n)
+    \<mapsto> (case s (var_bit_to_var (v, Suc n)) of Some x \<Rightarrow> x | None \<Rightarrow> One))"
+  show ?case using Suc
+    by(auto simp: fun_eq_iff var_to_operand_bit_eq_Some_iff numeral_3_eq_3 less_Suc_eq_le
+      split!: option.splits if_splits nat.splits
+      intro!: seq_terminates_when[where ?t1.0=3 and ?t2.0="4 * n" and ?s3.0="?s'"])
+qed
+
+fun copy_const_to_operand:: "nat \<Rightarrow> char \<Rightarrow> nat \<Rightarrow> IMP_Minus_com" where
+"copy_const_to_operand 0 op x = SKIP" |
+"copy_const_to_operand (Suc i) op x =
+   (operand_bit_to_var (op, i)) ::= (nth_bit x i) ;;
+    copy_const_to_operand i op x "
+
+lemma copy_const_to_operand_result:
+  "t_small_step_fun (4 * n) (copy_const_to_operand n op x, s)
+  = (SKIP, \<lambda>w. (case var_to_operand_bit w of
+    Some (op', i) \<Rightarrow> (if op' = op \<and> i < n then Some (nth_bit x i) else s w) |
+    _ \<Rightarrow> s w))"
+proof(induction n arbitrary: s)
+  case 0
+  then show ?case by (simp add: fun_eq_iff split: option.splits)
+next
+  case (Suc n)
+  let ?s' = "s(operand_bit_to_var (op, n) \<mapsto> nth_bit x n)"
+  show ?case using Suc
+    apply(auto simp: fun_eq_iff var_to_operand_bit_eq_Some_iff split!: option.splits if_splits
+      intro!: seq_terminates_when[where ?t1.0=1 and ?t2.0 ="4*n" and ?s3.0="?s'"])
+  using less_antisym by blast
+qed
+
+
+definition copy_atom_to_operand:: "nat \<Rightarrow> char \<Rightarrow> AExp.atomExp \<Rightarrow> IMP_Minus_com" where
+"copy_atom_to_operand n op a = (case a of
+  AExp.N x \<Rightarrow> copy_const_to_operand n op x |
+  AExp.V x \<Rightarrow> copy_var_to_operand n op x)"
+
+lemma copy_atom_to_operand_a_result:
+  "t_small_step_fun (4 * n) (copy_atom_to_operand n (a_chr) a,
+   IMP_State_To_IMP_Minus_with_operands_a_b s n b c)
+  = (SKIP, IMP_State_To_IMP_Minus_with_operands_a_b s n (AExp.atomVal a s) c)"
+  by (auto simp: copy_atom_to_operand_def fun_eq_iff copy_const_to_operand_result
+      copy_var_to_operand_result IMP_State_To_IMP_Minus_with_operands_a_b_def
+      var_to_operand_bit_eq_Some_iff
+      split!: option.splits AExp.atomExp.splits char.splits bool.splits nat.splits)
+
+lemma copy_atom_to_operand_b_result:
+  "t_small_step_fun (4 * n) (copy_atom_to_operand n (b_chr) a,
+   IMP_State_To_IMP_Minus_with_operands_a_b s n b c)
+  = (SKIP, IMP_State_To_IMP_Minus_with_operands_a_b s n b (AExp.atomVal a s))"
+  by(auto simp: copy_atom_to_operand_def fun_eq_iff copy_const_to_operand_result
+      copy_var_to_operand_result IMP_State_To_IMP_Minus_with_operands_a_b_def
+      var_to_operand_bit_eq_Some_iff
+      split!: option.splits AExp.atomExp.splits char.splits bool.splits)
+
+lemma copy_atom_to_operand_variables:
+  "set (enumerate_variables (copy_atom_to_operand n op a))
+    = { operand_bit_to_var (op, i) | i. i < n }
+    \<union> { var_bit_to_var (v, Suc i) | i v. i < n \<and> v \<in> set (vars a) }"
+  apply (induction n)
+  apply(cases a)
+    apply (auto simp: copy_atom_to_operand_def enumerate_variables_def)[1]
+   apply (auto simp: copy_atom_to_operand_def enumerate_variables_def)[1]
+  apply(cases a)
+   apply (auto simp: copy_atom_to_operand_def set_enumerate_variables_seq)
+  by(auto simp: enumerate_variables_def var_bit_to_var_neq_operand_bit_to_var[symmetric])
+
+definition assign_var_carry::
+  "nat \<Rightarrow> vname \<Rightarrow> nat \<Rightarrow> nat \<Rightarrow> nat \<Rightarrow> nat \<Rightarrow> IMP_Minus_com" where
+"assign_var_carry i v a b c z =
+  (var_bit_to_var (v, Suc i)) ::= (if a + b + c = 1 \<or> a + b + c = 3 then One else Zero) ;;
+  carry ::= (if a + b + c \<ge> 2 then One else Zero) ;;
+  zero ::= (if z = 0 \<and> (a + b + c = 0 \<or> a + b + c = 2) then Zero else One)"
+
+lemma result_of_assign_var_carry:
+  "t_small_step_fun 7 (assign_var_carry i v a b c z, s)
+    = (SKIP, s(var_bit_to_var (v, Suc i) \<mapsto> (if a + b + c = 1 \<or> a + b + c = 3 then One else Zero),
+     carry \<mapsto> (if a + b + c \<ge> 2 then One else Zero),
+      zero \<mapsto> (if z = 0 \<and> (a + b + c = 0 \<or> a + b + c = 2) then Zero else One)))"
+  by(auto simp: assign_var_carry_def t_small_step_fun_terminate_iff)
+
+definition full_adder:: "nat \<Rightarrow> vname \<Rightarrow> IMP_Minus_com" where
+"full_adder i v  = (
+let
+  assign = assign_var_carry i v;
+  op_a = operand_bit_to_var (a_chr, i);
+  op_b = operand_bit_to_var (b_chr, i)
+ in
+  IF op_a\<noteq>0 THEN (
+    IF op_b\<noteq>0 THEN (
+      IF carry\<noteq>0 THEN (
+        IF zero\<noteq>0 THEN assign 1 1 1 1
+                      ELSE assign 1 1 1 0)
+      ELSE (
+        IF zero\<noteq>0 THEN assign 1 1 0 1
+                      ELSE assign 1 1 0 0))
+    ELSE (
+      IF carry\<noteq>0 THEN (
+        IF zero\<noteq>0 THEN assign 1 0 1 1
+                      ELSE assign 1 0 1 0)
+      ELSE (
+        IF zero\<noteq>0 THEN assign 1 0 0 1
+                       ELSE assign 1 0 0 0)))
+  ELSE (
+    IF op_b\<noteq>0 THEN (
+      IF carry\<noteq>0 THEN (
+        IF zero\<noteq>0 THEN assign 0 1 1 1
+                      ELSE assign 0 1 1 0)
+      ELSE (
+        IF zero\<noteq>0 THEN assign 0 1 0 1
+                      ELSE assign 0 1 0 0))
+    ELSE (
+      IF carry\<noteq>0 THEN (
+        IF zero\<noteq>0 THEN assign 0 0 1 1
+                      ELSE assign 0 0 1 0)
+      ELSE (
+        IF zero\<noteq>0 THEN assign 0 0 0 1
+                      ELSE assign 0 0 0 0)))
+)"
+
+lemma full_adder_correct:
+  assumes 
+    "i = 0 \<longrightarrow> s carry = Some Zero \<and> s zero = Some Zero"
+    "i > 0 \<longrightarrow> s carry = Some (nth_carry (i - 1) a b) \<and> s zero = Some (zero_bit (a+b) i)"
+    "s (operand_bit_to_var (a_chr, i)) = Some (nth_bit a i)"
+    "s (operand_bit_to_var (b_chr, i)) = Some (nth_bit b i)"
+  shows "t_small_step_fun 11 (full_adder i v, s) = (SKIP,
+    s(var_bit_to_var (v, Suc i) \<mapsto> nth_bit (a + b) i, carry \<mapsto> nth_carry i a b, zero \<mapsto> zero_bit (a + b) (i + 1)))"
+  using assms
+  apply(simp add: full_adder_def Let_def t_small_step_fun_terminate_iff result_of_assign_var_carry)
+  apply(cases i)
+   apply (simp_all add: fun_eq_iff first_bit_of_add nth_bit_of_add zero_bit_rec)
+  done
+
+lemma full_adder_variables: "set (enumerate_variables (full_adder i v)) =
+  { operand_bit_to_var (a_chr, i), operand_bit_to_var (b_chr, i), var_bit_to_var (v, Suc i),
+    carry, zero}"
+  apply (subst larvs_set_enum[symmetric])
+  unfolding full_adder_def by (auto simp: Let_def assign_var_carry_def)
+
+lemma sequence_of_full_adders:
+  assumes
+    "s carry = Some Zero"
+    "s zero = Some Zero"
+    "\<forall>j < k. s (operand_bit_to_var (a_chr, j)) = Some (nth_bit a j)"
+    "\<forall>j < k. s (operand_bit_to_var (b_chr, j)) = Some (nth_bit b j)"
+  shows
+   "t_small_step_fun (13 * k) (com_list_to_seq (map (\<lambda>i. full_adder i v) [0..< k]), s)
+  = (SKIP, (\<lambda>w. (case var_to_var_bit w of
+    Some (w', Suc m) \<Rightarrow> (if w' = v \<and> m < k then Some (nth_bit (a + b) m) else s w) |
+    _ \<Rightarrow> (if w = carry \<and> k > 0 then Some (nth_carry (k-1) a b)
+          else if w = zero then Some (zero_bit (a+b) k)
+          else s w))))"
+  using assms
+proof(induction k)
+  case 0
+  with assms(1,2) show ?case by (auto simp: fun_eq_iff split: option.splits nat.splits)
+next
+  case (Suc k)
+  let ?s = 
+    "(\<lambda>w. case var_to_var_bit w of
+      Some (w', Suc m) \<Rightarrow> if w' = v \<and> m < k then Some (nth_bit (a + b) m) else s w
+    | _ \<Rightarrow> 
+      if w = carry \<and> 0 < k then Some (nth_carry (k - 1) a b) else
+      if w = zero then Some (zero_bit (a + b) k) 
+      else s w)"
+
+  from Suc.prems have
+    "\<forall>j<k. s (operand_bit_to_var (a_chr, j)) = Some (nth_bit a j)"
+    "\<forall>j<k. s (operand_bit_to_var (b_chr, j)) = Some (nth_bit b j)"
+    by auto
+  from Suc.IH[OF Suc.prems(1,2) this] 
+  have 1: "t_small_step_fun (13 * k) (com_list_to_seq (map (\<lambda>i. full_adder i v) [0..<k]), s) = (SKIP, ?s)"
+    by simp
+  let ?s2 =
+    "(\<lambda>w. case var_to_var_bit w of
+      Some (w', Suc m) \<Rightarrow> if w' = v \<and> m < Suc k then Some (nth_bit (a + b) m) else s w
+    | _ \<Rightarrow>
+      if w = carry \<and> 0 < Suc k then Some (nth_carry (Suc k - 1) a b) else 
+      if w = zero then Some (zero_bit (a + b) (Suc k))
+      else s w)"
+
+  have 2: "t_small_step_fun 11 ((full_adder k v), ?s) = (SKIP, ?s2)"
+    apply (subst full_adder_correct)
+    by (auto simp: Suc.prems fun_eq_iff var_to_var_bit_eq_Some_iff split!: if_splits option.splits nat.splits)
+  have "map (\<lambda>i. full_adder i v) [0..<Suc k] = (map (\<lambda>i. full_adder i v) [0..<k]) @ [full_adder k v]" by simp
+  with 1 2 show ?case
+    apply simp
+    apply (rule t_small_step_fun_com_list_to_seq_terminates)
+      apply auto
+    done
+qed
+
+definition write_zero where
+"write_zero n v = 
+  IF zero\<noteq>0 THEN 
+    (var_bit_to_var (v, 0)) ::= One
+   ELSE (var_bit_to_var (v, 0)) ::= Zero;;
+   carry ::= Zero ;;
+   zero ::= Zero"
+
+lemma result_write_zero: "t_small_step_fun 6
+     (write_zero n v,
+      \<lambda>w. case var_to_var_bit w of
+         Some (w', Suc m) \<Rightarrow>
+            
+            if w' = v \<and> m < n then Some (nth_bit c m)
+            else IMP_State_To_IMP_Minus_with_operands_a_b s n a b w
+       | _ \<Rightarrow>
+            if w = carry \<and> 0 < n then Some cv else
+            if w = zero then Some (zero_bit c n) else
+            IMP_State_To_IMP_Minus_with_operands_a_b s n a b w)
+         =
+    (SKIP,
+     \<lambda>w. case var_to_var_bit w of
+          None \<Rightarrow>
+            if w = carry then Some Zero else
+            if w = zero then Some Zero else
+            IMP_State_To_IMP_Minus_with_operands_a_b s n a b w
+        | Some (w', m) \<Rightarrow> 
+            if w' = v then (
+              case m of 0 \<Rightarrow> Some (zero_bit ((s(v := c)) w') n)
+            | Suc m \<Rightarrow>
+                 if m < n then Some (nth_bit c m) else 
+                 IMP_State_To_IMP_Minus_with_operands_a_b s n a b w)
+            else IMP_State_To_IMP_Minus_with_operands_a_b s n a b w)"
+  unfolding write_zero_def
+  by (auto simp: numeral_eq_Suc simp: fun_eq_iff var_to_var_bit_eq_Some_iff split: if_splits option.splits nat.splits)
+
+lemma write_zero_vars[simp]: 
+  "set (enumerate_variables (write_zero n v)) = {zero, carry, var_bit_to_var (v,0)}"
+  unfolding write_zero_def
+  apply (subst larvs_set_enum[symmetric])
+  by auto
+
+definition adder:: "nat \<Rightarrow> vname \<Rightarrow> IMP_Minus_com" where
+"adder n v = 
+  com_list_to_seq (map (\<lambda>i. full_adder i v) [0..< n]) ;; 
+  write_zero n v
+"
+
+lemma result_of_adder:
+  assumes "a + b < 2 ^ n"
+  shows "t_small_step_fun (13 * n + 13) (adder n v,
+    IMP_State_To_IMP_Minus_with_operands_a_b s n a b)
+    = (SKIP, IMP_State_To_IMP_Minus_with_operands_a_b (s(v := a + b)) n a b)"
+  using assms
+  apply(simp only: adder_def)
+  apply(rule seq_terminates_when[OF _  sequence_of_full_adders[where a=a and b=b],of _ 6])
+  apply (auto simp: fun_eq_iff var_to_var_bit_eq_Some_iff IMP_State_To_IMP_Minus_with_operands_a_b_def
+      split!: option.splits if_splits)
+  apply (subst result_write_zero)
+  apply (auto simp: IMP_State_To_IMP_Minus_with_operands_a_b_def split: if_splits option.splits nat.splits)
+  done
+
+definition binary_adder:: "nat \<Rightarrow> vname \<Rightarrow> AExp.atomExp \<Rightarrow> AExp.atomExp \<Rightarrow> IMP_Minus_com" where
+"binary_adder n v a b =
+  copy_atom_to_operand n (a_chr) a ;;
+  (copy_atom_to_operand n (b_chr) b ;;
+  (adder n v ;;
+  (copy_atom_to_operand n (a_chr) (AExp.N 0) ;;
+  copy_atom_to_operand n (b_chr) (AExp.N 0))))"
+
+lemma binary_adder_correct:
+  assumes "n > 0"
+    "AExp.atomVal a s + AExp.atomVal b s < 2 ^ n"
+  shows "t_small_step_fun (50 * (n + 1)) (binary_adder n v a b,
+    IMP_State_To_IMP_Minus s n)
+    = (SKIP, IMP_State_To_IMP_Minus (s(v := AExp.atomVal a s + AExp.atomVal b s)) n)"
+  using seq_terminates_when'[OF copy_atom_to_operand_a_result[where ?n=n]
+      seq_terminates_when'[OF copy_atom_to_operand_b_result
+      seq_terminates_when'[OF result_of_adder
+      seq_terminates_when'[OF copy_atom_to_operand_a_result copy_atom_to_operand_b_result]]]]
+  assms
+  by(fastforce simp: binary_adder_def IMP_State_To_IMP_Minus_def)
+
+
+section \<open>Subtraction\<close>
+
+definition assign_var_carry_sub::
+  "nat \<Rightarrow> vname \<Rightarrow> nat \<Rightarrow> nat \<Rightarrow> nat \<Rightarrow> nat \<Rightarrow> IMP_Minus_com" where
+"assign_var_carry_sub i v a b c z =
+  (var_bit_to_var (v, Suc i)) ::= 
+    (if b + c = 0 \<or> b + c = 2 then (if a = 1 then One else Zero)
+     else (if b + c = 1 \<and> a = 0 then One else Zero)) ;;
+  carry ::= (if a < b + c then One else Zero);;
+  zero ::= (if z = 0 \<and> ((a + b + c = 0) \<or> (b + c = 2 \<and> a = 0) \<or> (b + c = 1 \<and> a = 1)) then Zero else One)"
+
+lemma result_of_assign_var_carry_sub:
+  "t_small_step_fun 7 (assign_var_carry_sub i v a b c z, s)
+    = (SKIP, s(var_bit_to_var (v, Suc i) \<mapsto> (if b + c = 0 \<or> b + c = 2 then (if a = 1 then One else Zero)
+    else (if b + c = 1 \<and> a = 0 then One else Zero)),
+     carry \<mapsto>  (if a < b + c then One else Zero), 
+     zero \<mapsto> (if z = 0 \<and> ((a + b + c = 0) \<or> (b + c = 2 \<and> a = 0) \<or> (b + c = 1 \<and> a = 1)) then Zero else One)))"
+  by(auto simp: assign_var_carry_sub_def t_small_step_fun_terminate_iff)
+
+definition full_subtractor:: "nat \<Rightarrow> vname \<Rightarrow> IMP_Minus_com" where
+"full_subtractor i v  = (
+let
+  assign = assign_var_carry_sub i v;
+  op_a = operand_bit_to_var (a_chr, i);
+  op_b = operand_bit_to_var (b_chr, i)
+  in
+  IF op_a\<noteq>0 THEN (
+    IF op_b\<noteq>0 THEN (
+      IF carry\<noteq>0 THEN (
+        IF zero\<noteq>0 THEN assign 1 1 1 1
+                      ELSE assign 1 1 1 0)
+      ELSE (
+        IF zero\<noteq>0 THEN assign 1 1 0 1
+                      ELSE assign 1 1 0 0))
+    ELSE (
+      IF carry\<noteq>0 THEN (
+        IF zero\<noteq>0 THEN assign 1 0 1 1
+                      ELSE assign 1 0 1 0)
+      ELSE (
+        IF zero\<noteq>0 THEN assign 1 0 0 1
+                       ELSE assign 1 0 0 0)))
+  ELSE (
+    IF op_b\<noteq>0 THEN (
+      IF carry\<noteq>0 THEN (
+        IF zero\<noteq>0 THEN assign 0 1 1 1
+                      ELSE assign 0 1 1 0)
+      ELSE (
+        IF zero\<noteq>0 THEN assign 0 1 0 1
+                      ELSE assign 0 1 0 0))
+    ELSE (
+      IF carry\<noteq>0 THEN (
+        IF zero\<noteq>0 THEN assign 0 0 1 1
+                      ELSE assign 0 0 1 0)
+      ELSE (
+        IF zero\<noteq>0 THEN assign 0 0 0 1
+                      ELSE assign 0 0 0 0)))
+)"
+
+lemma full_subtractor_correct_no_underflow:
+  assumes "a \<ge> b"
+    "i = 0 \<longrightarrow> s carry = Some Zero \<and> s zero = Some Zero"
+    "i > 0 \<longrightarrow> s carry = Some (nth_carry_sub (i - 1) a b) \<and> s zero = Some (zero_bit (a-b) i)"
+    "s (operand_bit_to_var (a_chr, i)) = Some (nth_bit a i)"
+    "s (operand_bit_to_var (b_chr, i)) = Some (nth_bit b i)"
+  shows "t_small_step_fun 11 (full_subtractor i v, s) = (SKIP,
+    s(var_bit_to_var (v, Suc i) \<mapsto> nth_bit (a - b) i, carry \<mapsto> nth_carry_sub i a b, zero \<mapsto> zero_bit (a - b) (i + 1)))"
+  using assms
+  apply(simp add: full_subtractor_def Let_def t_small_step_fun_terminate_iff result_of_assign_var_carry_sub split: nat.splits)
+  apply(cases i)
+   apply (simp_all add: fun_eq_iff first_bit_of_sub_n_no_underflow nth_bit_of_sub_n_no_underflow Let_def zero_bit_rec)
+  done
+
+lemma full_subtractor_variables: "set (enumerate_variables (full_subtractor i v)) =
+  { operand_bit_to_var (a_chr, i), operand_bit_to_var (b_chr, i), var_bit_to_var (v, Suc i),
+    carry, zero}"
+  apply (subst larvs_set_enum[symmetric])
+  unfolding full_subtractor_def Let_def
+  by (auto simp: assign_var_carry_sub_def)
+
+lemma sequence_of_full_subtractors_no_underflow:
+  assumes "a \<ge> b"
+    "s carry = Some Zero"
+    "s zero = Some Zero"
+    "\<forall>j < n. s (operand_bit_to_var (a_chr, j)) = Some (nth_bit a j)"
+    "\<forall>j < n. s (operand_bit_to_var (b_chr, j)) = Some (nth_bit b j)"
+  shows
+   "t_small_step_fun (13 * n) (com_list_to_seq (map (\<lambda>i. full_subtractor i v) [0..< n]), s)
+  = (SKIP, (\<lambda>w. (case var_to_var_bit w of
+    Some (w', Suc m) \<Rightarrow> (if w' = v \<and> m < n then Some (nth_bit (a - b) m) else s w) |
+    _ \<Rightarrow> (if w = carry \<and> n > 0 then Some (nth_carry_sub (n - 1) a b)
+          else if w = zero then Some (zero_bit (a-b) n)
+          else s w))))"
+  using assms
+proof(induction n)
+  case 0
+  with assms(1,2) show ?case by (auto simp: fun_eq_iff split: option.splits nat.splits)
+next
+  case (Suc n)
+  have "t_small_step_fun (13 + 13 * n)
+   (com_list_to_seq ((map (\<lambda>i. full_subtractor i v) [0..< n]) @ [full_subtractor n v]), s)
+    = (SKIP, (\<lambda>w. (case var_to_var_bit w of
+      Some (w', Suc m) \<Rightarrow> (if w' = v \<and> m < Suc n then Some (nth_bit (a - b) m) else s w) |
+      _ \<Rightarrow> 
+        (if w = carry \<and> Suc n > 0 then Some (nth_carry_sub n a b) else
+         if w = zero then Some (zero_bit (a-b) (Suc n))
+         else s w))))"
+    apply(rule t_small_step_fun_com_list_to_seq_terminates[OF _ Suc.IH
+          iffD2[OF com_list_to_seq_of_length_one_terminates_iff[where ?t="12"]]])
+    using Suc  apply(auto)
+    apply(subst full_subtractor_correct_no_underflow)
+    using Suc
+    apply (auto simp add: fun_eq_iff var_to_var_bit_eq_Some_iff split!: option.splits nat.splits if_splits)
+    done
+  thus ?case by auto
+qed
+
+lemma sequence_of_full_subtractors_with_underflow:
+  assumes "a < b"
+    "a < 2^n" "b < 2^n"
+    "s carry = Some Zero"
+    "s zero = Some Zero"
+    "\<forall>j < n. s (operand_bit_to_var (a_chr, j)) = Some (nth_bit a j)"
+    "\<forall>j < n. s (operand_bit_to_var (b_chr, j)) = Some (nth_bit b j)"
+  shows
+   "t_small_step_fun (13 * n) (com_list_to_seq (map (\<lambda>i. full_subtractor i v) [0..< n]), s)
+  = (SKIP, (\<lambda>w. (case var_to_var_bit w of
+    Some (w', Suc m) \<Rightarrow> (if w' = v \<and> m < n then Some (nth_bit (2^n + a - b) m) else s w) |
+    _ \<Rightarrow> (if w = carry \<and> n > 0 then Some One
+          else if w = zero then Some (zero_bit (2^n + a - b) n)
+          else s w))))"
+proof -
+  have "\<forall>j < n. s (operand_bit_to_var (a_chr, j)) = Some (nth_bit (2 ^ n + a) j)"
+    using nth_bit_add_out_of_range[OF \<open>a < 2^n\<close>]
+      \<open>\<forall>j < n. s (operand_bit_to_var (a_chr, j)) = Some (nth_bit a j)\<close> by simp
+  moreover have "2 ^ n + a > b" using \<open>b < 2^n\<close> by simp
+  ultimately have "t_small_step_fun (13 * n)
+                       (com_list_to_seq (map (\<lambda>i. full_subtractor i v) [0..< n]), s)
+  = (SKIP, (\<lambda>w. (case var_to_var_bit w of
+    Some (w', Suc m) \<Rightarrow> (if w' = v \<and> m < n then Some (nth_bit (2^n + a - b) m) else s w) |
+    _ \<Rightarrow> (if w = carry \<and> n > 0 then Some (nth_carry_sub (n - 1) (2^n + a) b) else
+          if w = zero then Some (zero_bit (2^n + a - b) n)
+          else s w))))"
+    using sequence_of_full_subtractors_no_underflow[where ?a="2^n + a" and ?b=b] assms
+    by(auto simp: fun_eq_iff)
+  thus ?thesis using assms nth_carry_sub_underflow by auto
+qed
+
+definition underflow_handler:: "nat \<Rightarrow> vname \<Rightarrow> IMP_Minus_com" where
+"underflow_handler n v = (
+IF carry\<noteq>0 THEN 
+  ((carry ::= Zero ;;
+   zero ::= Zero);;
+  binary_assign_constant n v 0)
+ELSE SKIP)"
+
+text \<open>Intro rules for easy reasoning:\<close>
+
+lemma seq_intro:
+ "t_small_step_fun n1 (c1,s) = (SKIP,s2) \<Longrightarrow> 
+  t_small_step_fun n2 (c2,s2) = (SKIP,s3) \<Longrightarrow>
+  t = n1 + n2 + 1 \<Longrightarrow>  
+  t_small_step_fun t (c1;;c2,s) = (SKIP,s3)"
+  apply (auto simp add: t_small_step_fun_decomposition t_small_step_fun_small_step_fun tsmall_seq)
+  by (metis IMP_Minus_Small_StepT.small_step_fun.simps(3)
+      t_small_step_fun_decomposition t_small_step_fun_small_step_fun
+      tsmall_seq)
+
+lemma assign_intro:
+"t_small_step_fun (Suc 0) (c ::= b,s) = (SKIP,s(c := Some b))"
+  by simp
+
+lemma ifTrue_intro:
+"s b \<noteq> Some Zero \<Longrightarrow> t_small_step_fun n (c, s) = (SKIP,s2) \<Longrightarrow> n2 = Suc n \<Longrightarrow>
+   t_small_step_fun n2 (IF b\<noteq>0 THEN c ELSE c2,s) = (SKIP, s2)"
+  by simp
+
+lemma ifFalse_intro:
+"s b = Some Zero \<Longrightarrow> t_small_step_fun n (c2, s) = (SKIP,s2) \<Longrightarrow> n2 = Suc n \<Longrightarrow>
+   t_small_step_fun n2 (IF b\<noteq>0 THEN c ELSE c2,s) = (SKIP, s2)"
+  by simp
+
+
+lemmas intros = seq_intro assign_intro 
+
+
+lemma result_underflow_handler_carry: "s carry \<noteq> Some Zero \<Longrightarrow>
+ t_small_step_fun (3 * n + 8)
+     (underflow_handler n v, s) =
+    (SKIP, (\<lambda>w. case var_to_var_bit w of
+          None \<Rightarrow>
+            if w = carry then Some Zero
+            else if w = zero then Some Zero
+            else s w
+          | Some (w', m) \<Rightarrow>
+              if w' = v then case m of
+                0 \<Rightarrow> Some (zero_bit 0 n)
+              | Suc m \<Rightarrow> if m < n then Some (nth_bit 0 m) else s w
+              else s w))"
+  unfolding underflow_handler_def
+  apply (auto  intro!:  intros ifTrue_intro)
+  apply (subst t_small_step_fun_increase_time[OF _ result_of_binary_assign_constant])
+   apply (auto split!: if_splits option.splits nat.splits)
+  done
+
+lemma result_underflow_handler_carry_Skip: "s carry = Some Zero \<Longrightarrow>
+  t_small_step_fun (3 * n + 8)
+     (underflow_handler n v, s) =
+    (SKIP, s)"
+  unfolding underflow_handler_def
+  by (auto intro!: intros ifFalse_intro)  
+
+definition subtract_handle_underflow::
+  "nat \<Rightarrow> vname \<Rightarrow> IMP_Minus_com" where
+"subtract_handle_underflow n v =
+  com_list_to_seq (map (\<lambda>i. full_subtractor i v) [0..<n]) ;;
+  (underflow_handler n v;;
+  write_zero n v)"
+
+lemma "Zero = zero_bit 0 n"
+  using zero_bit_one by fastforce
+
+lemma result_of_subtract_handle_underflow:
+  assumes "n > 0" "a < 2 ^ n" "b < 2 ^ n"
+  shows "t_small_step_fun (16 * n + 16) (subtract_handle_underflow n v,
+    IMP_State_To_IMP_Minus_with_operands_a_b s n a b)
+    = (SKIP, IMP_State_To_IMP_Minus_with_operands_a_b (s(v := a - b)) n a b)"
+proof(cases "a < b")
+  case True
+  with assms show ?thesis
+    apply (simp only: subtract_handle_underflow_def)
+    apply (rule seq_terminates_when[OF _  sequence_of_full_subtractors_with_underflow[where ?a=a and ?b=b], of _ "3*n + 15"]) 
+            apply auto
+    apply (rule seq_terminates_when[of "3*n + 8" "6"])
+      apply auto
+    apply (subst result_underflow_handler_carry)
+     apply (auto)
+    unfolding write_zero_def
+    apply (auto  simp: numeral_eq_Suc simp: fun_eq_iff var_to_var_bit_eq_Some_iff 
+        IMP_State_To_IMP_Minus_with_operands_a_b_of_changed_s_neq_iff split: if_splits option.splits nat.splits)
+     defer using zero_bit_one apply fastforce
+    using IMP_State_To_IMP_Minus_with_operands_a_b_of_changed_s_neq_iff
+    by (metis not_Some_eq)
+next
+  case False
+  with assms show ?thesis
+    apply(simp only: subtract_handle_underflow_def)
+    apply(rule seq_terminates_when[OF _  sequence_of_full_subtractors_no_underflow[where ?a=a and ?b=b],
+          where ?t2.0="3 * n + 15"])
+          apply auto
+    apply (rule seq_terminates_when[of "3*n+8" 6])
+    apply auto
+     apply (subst result_underflow_handler_carry_Skip)
+      apply auto
+    unfolding write_zero_def
+     apply (auto simp: numeral_eq_Suc simp: fun_eq_iff var_to_var_bit_eq_Some_iff 
+        IMP_State_To_IMP_Minus_with_operands_a_b_of_changed_s_neq_iff split: if_splits option.splits nat.splits)
+    apply (metis One_nat_def assms(2,3) nth_carry_sub_no_underflow
+        verit_comp_simplify1(3))
+     using nth_carry_sub_no_underflow[OF _ \<open>a < 2 ^ n\<close> \<open>b < 2 ^ n\<close>]
+    apply(auto simp:  IMP_State_To_IMP_Minus_with_operands_a_b_of_changed_s_neq_iff
+        var_to_var_bit_eq_Some_iff
+        split!: option.splits if_splits)
+     by(auto simp: IMP_State_To_IMP_Minus_with_operands_a_b_def)
+qed
+
+lemma subtract_handle_underflow_variables:
+  "set (enumerate_variables (subtract_handle_underflow n v))
+  = { operand_bit_to_var (op, i) | i op. i < n \<and> (op = a_chr \<or> op = b_chr) }
+    \<union> { var_bit_to_var (v, i) | i. i \<le> n }
+    \<union> { carry, zero }"
+  apply (auto simp: subtract_handle_underflow_def gr0_conv_Suc
+       set_enumerate_variables_seq com_list_to_seq_variables full_subtractor_variables
+       set_enumerate_variables_if underflow_handler_def)
+  done
+
+definition binary_subtractor:: "nat \<Rightarrow> vname \<Rightarrow> AExp.atomExp \<Rightarrow> AExp.atomExp \<Rightarrow> IMP_Minus_com" where
+"binary_subtractor n v a b =
+  copy_atom_to_operand n (a_chr) a ;;
+  (copy_atom_to_operand n (b_chr) b ;;
+  (subtract_handle_underflow n v ;;
+  (copy_atom_to_operand n (a_chr) (AExp.N 0) ;;
+  copy_atom_to_operand n (b_chr) (AExp.N 0))))"
+
+lemma binary_subtractor_correct:
+  assumes "n > 0"
+    "AExp.atomVal a s < 2 ^ n" "AExp.atomVal b s < 2 ^ n"
+  shows "t_small_step_fun (50 * (n + 1)) (binary_subtractor n v a b,
+    IMP_State_To_IMP_Minus s n)
+    = (SKIP, IMP_State_To_IMP_Minus (s(v := AExp.atomVal a s - AExp.atomVal b s)) n)"
+  unfolding binary_subtractor_def
+  using assms
+  apply (auto simp: IMP_State_To_IMP_Minus_def  intro!: intros copy_atom_to_operand_a_result copy_atom_to_operand_b_result 
+      result_of_subtract_handle_underflow )
+  apply (subst t_small_step_fun_increase_time[OF _ copy_atom_to_operand_b_result])
+   apply auto
+  done
+
+text \<open> The two copy_atom_to_operand which don't have any effect on the output are only a hack to
+       ensure that all bits of all variables in IMP occur in IMP- \<close>
+
+fun assign_shifted_bits:: "nat \<Rightarrow> vname \<Rightarrow> IMP_Minus_com" where
+"assign_shifted_bits 0 v = SKIP" |
+"assign_shifted_bits (Suc i) v = (IF operand_bit_to_var ((a_chr), Suc i)\<noteq>0 THEN
+    (var_bit_to_var (v, i)) ::= One
+  ELSE
+    (var_bit_to_var (v, i)) ::= Zero) ;;
+  assign_shifted_bits i v"
+
+lemma result_of_assign_shifted_bits:
+  "t_small_step_fun (3 * k) (assign_shifted_bits k v, s) = (SKIP, (\<lambda>w.
+    (case var_to_var_bit w of Some(v', i) \<Rightarrow> (if v' = v \<and> i < k then
+      (if s (operand_bit_to_var (a_chr, Suc i)) \<noteq> Some Zero then Some One else Some Zero)
+      else s w) |
+      _ \<Rightarrow> s w)))"
+proof(induction k arbitrary: s)
+  case (Suc k)
+  have *: "t_small_step_fun 2 (IF operand_bit_to_var ((a_chr), Suc k)\<noteq>0 THEN
+      (var_bit_to_var (v, k)) ::= One
+   ELSE
+      (var_bit_to_var (v, k)) ::= Zero, s) = (SKIP, s(var_bit_to_var (v, k) \<mapsto>
+        (if s (operand_bit_to_var (a_chr, Suc k)) \<noteq> Some Zero then One else Zero)))"
+    by(auto simp: numeral_2_eq_2)
+  show ?case
+    using seq_terminates_when[OF _ * Suc.IH, where ?t="3 + 3 * k"]
+    apply (auto simp: fun_eq_iff var_to_var_bit_eq_Some_iff split: option.splits)
+    using var_bit_to_var_neq_operand_bit_to_var by (metis operand_bit_to_var.simps)+
+qed (auto simp: fun_eq_iff split: option.splits)
+
+lemma assign_shifted_bits_variables: "set (enumerate_variables (assign_shifted_bits k v))
+  = { var_bit_to_var (v, i) | i. i < k } \<union> { operand_bit_to_var (a_chr, i) | i. i > 0 \<and> i \<le> k }"
+  apply(induction k)
+   apply(auto simp: set_enumerate_variables_seq set_enumerate_variables_if)
+  done
+
+definition assignment_to_binary:: "nat \<Rightarrow> vname \<Rightarrow> AExp.aexp \<Rightarrow> IMP_Minus_com" where
+"assignment_to_binary n v aexp = (case aexp of
+  AExp.A a \<Rightarrow> binary_adder n v a (AExp.N 0) |
+  AExp.Plus a b \<Rightarrow> binary_adder n v a b |
+  AExp.Sub a b \<Rightarrow> binary_subtractor n v a b)"
+
+\<^marker>\<open>title "lem:bitblastExpr"\<close>
+lemma assignment_to_binary_correct:
+  assumes "n > 0"  "AExp.aval a s < 2 ^ n" "\<forall>v. s v < 2 ^ n" "max_const a < 2 ^ n"
+  shows
+    "t_small_step_fun (50 * (n + 1))
+       (assignment_to_binary n v a,
+        IMP_State_To_IMP_Minus s n)
+  = (SKIP, IMP_State_To_IMP_Minus (s(v := AExp.aval a s)) n)"
+using assms binary_adder_correct  proof(cases a)
+  case (Sub x31 x32)
+  then show ?thesis
+    apply(simp add: assignment_to_binary_def)
+    apply(rule binary_subtractor_correct[simplified])
+    using assms by(cases x31; cases x32; auto)+
+qed (auto simp: assignment_to_binary_def)
+
+lemma assignment_to_binary_variables:
+  "n > 0 \<Longrightarrow> set (enumerate_variables (assignment_to_binary n v a)) \<subseteq>
+    { var_bit_to_var (w, i) | w i. i \<le> n \<and> (w = v \<or> w \<in> set (vars a)) }
+    \<union> { operand_bit_to_var (op, i) | op i. i < n \<and> (op = a_chr \<or> op = b_chr) }
+    \<union> { carry, zero }"
+  apply(cases a)
+  apply(auto simp: assignment_to_binary_def binary_adder_def set_enumerate_variables_seq
+      copy_atom_to_operand_variables adder_def com_list_to_seq_variables full_adder_variables
+    binary_subtractor_def subtract_handle_underflow_variables
+    split: atomExp.splits)
+  done
+  
+
+end
