IMP-/IMP_To_IMP-/IMP_To_IMP_Minus.thy
@@ -1,0 +1,410 @@
+\<^marker>\<open>creator Florian Keßler\<close>
+\<^marker>\<open>contributors Mohammad Abdulaziz, Bilel Ghorbel\<close>
+
+section "IMP to IMP-"
+
+theory IMP_To_IMP_Minus
+  imports "IMP.Big_StepT" Binary_Operations
+begin
+
+text \<open> We give a reduction from IMP to IMP-. The reduction works by bit blasting each register
+       of IMP into several registers in IMP- each holding a single bit. Arithmetic operations
+       and assignment in IMP are replaced by the binary operations defined in the Binary Operations
+       theory. For WHILE and IF, we replace the condition of a single register's content being
+       non-zero by checking whether any of the bits in the translated state is non-zero. \<close>
+
+fun IMP_To_IMP_Minus:: "IMP_com \<Rightarrow> nat \<Rightarrow> IMP_Minus_com" where
+"IMP_To_IMP_Minus Com.SKIP n = SKIP" |
+"IMP_To_IMP_Minus (Com.Assign v aexp) n = assignment_to_binary n v aexp" |
+"IMP_To_IMP_Minus (Com.Seq c1 c2) n =
+  (IMP_To_IMP_Minus c1 n ;; IMP_To_IMP_Minus c2 n )" |
+"IMP_To_IMP_Minus (Com.If v c1 c2) n = (IF (var_bit_to_var (v, 0))\<noteq>0 THEN
+  IMP_To_IMP_Minus c1 n ELSE IMP_To_IMP_Minus c2 n)" |
+"IMP_To_IMP_Minus (Com.While v c) n = (WHILE (var_bit_to_var (v, 0))\<noteq>0 DO
+  IMP_To_IMP_Minus c n)"
+
+lemma finite_range_stays_finite: "(c1, s1) \<Rightarrow>\<^bsup>t\<^esup> s2 \<Longrightarrow> finite (range s1)
+  \<Longrightarrow> finite (range s2)"
+  apply(induction c1 s1 t s2 rule: big_step_t_induct)
+  apply auto
+  by (metis Un_infinite image_Un sup_top_right)
+
+unbundle no IMP_Minus_Com.com_syntax
+unbundle Com.com_syntax
+
+lemma Max_insert_le_when:
+  "\<lbrakk>finite (range (s :: vname \<Rightarrow> nat)); y < r;  Max (range s) < r\<rbrakk> \<Longrightarrow> Max (range (s(x := y))) < r"
+proof(goal_cases)
+  case 1
+  hence "finite (s ` {xa. xa \<noteq> x})"
+    using finite_nat_set_iff_bounded
+    by auto
+  moreover have "s ` {xa. xa \<noteq> x} \<noteq> {}"
+    using 1
+    by auto
+  moreover have "max y (Max (s ` {xa. xa \<noteq> x})) < r"
+    using 1
+    apply(subst max_less_iff_conj)
+    apply(subst Max_less_iff)
+    using finite_nat_set_iff_bounded
+    by auto
+  ultimately show ?case
+    by simp
+qed
+
+\<^marker>\<open>title "thm:spaceConsume"\<close>
+lemma IMP_space_growth:
+  "\<lbrakk>(c1, s1) \<Rightarrow>\<^bsup>t\<^esup> s2; finite (range s1);
+    max (Max (range s1)) (max_const c1) < 2 ^ k\<rbrakk> \<Longrightarrow>
+    (finite (range s2) \<and> Max (range s2) < (2 :: nat) ^ (k + t))"
+proof(induction c1 s1 t s2 arbitrary: k rule: big_step_t_induct)
+  case (Skip s)
+  thus ?case
+  by (smt add_lessD1 le_less_trans le_simps max_def mult_2 mult_Suc_right not_le plus_1_eq_Suc
+      power.simps power.simps power_add)
+next
+  case (Assign x a s)
+  hence "AExp.aval a s < 2 * 2 ^ k"
+    by (auto intro!: aval_le_when)
+  hence "Max (range (s(x := aval a s))) < 2 ^ (k + Suc (Suc 0))"
+    using Assign
+    by (fastforce simp: eval_nat_numeral intro!: trans_less_add2 Max_insert_le_when)
+  thus ?case using Assign
+    using finite_range_stays_finite
+    by blast
+next
+  case (Seq c1 s1 x s2 c2 y s3 z)
+  hence "finite (range s2)"
+    using finite_range_stays_finite
+    by blast
+  hence "s2 a < 2 ^ (k + x)" for a
+    using Seq \<open>finite (range s1)\<close> \<open>finite (range s2)\<close>
+    by auto
+  have "max_const c2  < 2 ^ k"
+    using Seq
+    by simp
+  hence "max_const c2 < (2 :: nat) ^ (k + x)"
+    using bigstep_progress Seq
+    by (auto simp: eval_nat_numeral intro: le_less_trans less_imp_le_nat  n_less_n_mult_m)
+  hence "s3 a < (2 :: nat) ^ (k + x + y)" for a using Seq \<open>finite (range s2)\<close>
+    by fastforce
+  moreover have "finite (range s3)"
+    using Seq.hyps(2) \<open>finite (range s2)\<close> finite_range_stays_finite
+    by blast
+  ultimately show ?case using Seq
+    by (auto simp: add.assoc eval_nat_numeral)
+next
+  case (WhileTrue s1 b c x s2 y s3 z)
+  hence "finite (range s2)" using finite_range_stays_finite by blast
+  hence "s2 a < 2 ^ (k + x)" for a
+    using WhileTrue \<open>finite (range s1)\<close> \<open>finite (range s2)\<close>
+    by auto
+  have "max_const (WHILE b\<noteq>0 DO c)  < 2 ^ k"
+    using WhileTrue
+    by simp
+  hence "max_const (WHILE b\<noteq>0 DO c) < (2 :: nat) ^ (k + x)"
+    by (metis One_nat_def WhileTrue.hyps(2) bigstep_progress le_less_trans lessI
+        less_add_same_cancel1 less_imp_le_nat numeral_2_eq_2 power_strict_increasing_iff)
+  hence "\<forall>a. s3 a < (2 :: nat) ^ (k + x + y)"
+    using WhileTrue \<open>finite (range s2)\<close>
+    by fastforce
+  moreover have "finite (range s3)"
+    using WhileTrue.hyps(3) \<open>finite (range s2)\<close> finite_range_stays_finite
+    by blast
+  ultimately show ?case using WhileTrue
+    by (auto simp: group_cancel.add1 mult_2 trans_less_add2)
+qed (auto simp: numeral_2_eq_2 trans_less_add1)
+
+lemma power_of_two_minus: "2 ^ a * c < 2 ^ b \<Longrightarrow> c < (2 :: nat) ^ (b - a)"
+proof(induction a arbitrary: c)
+  case (Suc a)
+  hence "2 * c < 2 ^ (b - a)" by auto
+  thus ?case
+    by (metis One_nat_def Suc_diff_Suc bot_nat_0.not_eq_extremum less_Suc0
+              nat_mult_less_cancel_disj numeral_2_eq_2 power_0 power_Suc zero_less_diff zero_less_power)
+qed auto
+
+lemma power_of_two_increase_exponent_le: "(2 :: nat) ^ (a + b) * c < r \<Longrightarrow> 2 ^ a * c < r"
+  by(auto intro: dual_order.strict_trans2)
+
+lemma move_exponent_to_rhs: "c < (2 :: nat) ^ (a - b) \<Longrightarrow> 2 ^ b * c < 2 ^ a"
+  by (smt One_nat_def diff_mult_distrib2 gr_zeroI less_Suc0
+      linordered_semidom_class.add_diff_inverse mult_eq_0_iff order.asym power.simps(1)
+      power_add power_eq_0_iff zero_less_diff zero_neq_numeral)
+
+subsection \<open>Correctness\<close>
+
+text \<open>First direction of the correctness statement. We show that when an IMP program run from a
+      state where all values are bounded terminates in some state, then the translated IMP- program
+      started on the translated initial state will terminate in the translated final state, after
+      a number of steps that is polynomially bigger than the number of steps the IMP program run
+      for. The constants appearing in the polynomial bound have no significance.  \<close>
+
+\<^marker>\<open>title "lem:bitblastProgram"\<close>
+lemma IMP_To_IMP_Minus:
+  assumes
+    "(c1 :: IMP_com, s1) \<Rightarrow>\<^bsup>t\<^esup> s2"
+    "finite (range s1)"
+    "n > t"
+    "((2 :: nat) ^ t) * (max (Max (range s1)) (max_const c1)) < 2 ^ n"
+  shows
+    "t_small_step_fun (100 * n * (t - 1) + 50)
+      (IMP_To_IMP_Minus c1 n, IMP_State_To_IMP_Minus s1 n)
+     = (SKIP, IMP_State_To_IMP_Minus s2 n)"
+  using assms
+proof(induction c1 s1 t s2 rule: big_step_t_induct)
+  case (Assign x a s)
+  moreover hence "s v < (2 :: nat) ^ n" for v
+    using Max_range_le_then_element_le[where ?s=s and ?x="2^n" and ?y=v] by fastforce
+  ultimately show ?case
+    apply(subst t_small_step_fun_increase_time[where ?t="50 * (n + 1)"])
+    by (auto simp: aval_le_when IMP_State_To_IMP_Minus_def fun_eq_iff
+             intro!: assignment_to_binary_correct[simplified]
+             split!: option.splits)
+next
+  case (Seq c1 s1 x s2 c2 y s3 z)
+  hence "(2 :: nat) ^ x \<le> 2 ^ z" by simp
+  hence "((2 :: nat) ^ x) * max (Max (range s1)) (max_const (c1 ;; c2)) < 2 ^ n"
+    using Seq(8)
+    by (meson leD leI less_le_trans mult_less_cancel2)
+  hence "2 ^ x * max (Max (range s1)) (max_const c1) < 2 ^ n"
+    by (simp add: nat_mult_max_right)
+  have "max (Max (range s1)) (max_const (c1)) < 2 ^ (n - z)"
+    using power_of_two_minus Seq.prems(3)
+    by fastforce
+  have "Max (range s2) < 2 ^ (n - y)"
+    using
+      IMP_space_growth[OF \<open>(c1, s1) \<Rightarrow>\<^bsup> x \<^esup> s2\<close> \<open>finite (range s1)\<close>
+                                \<open>max (Max (range s1)) (max_const (c1)) < 2 ^ (n - z)\<close>]
+      \<open>z = x + y\<close> \<open>n > z \<close>
+    by auto
+  hence "2 ^ y * Max (range s2) < 2 ^ n"
+    using move_exponent_to_rhs
+    by blast
+ moreover have "2 ^ y * max_const c2 < 2 ^ n"
+    using \<open>z = x + y\<close> \<open>2 ^ z * max (Max (range s1)) (max_const (c1;; c2)) < 2 ^ n\<close>
+          power_of_two_increase_exponent_le[where ?b=x]
+    by(auto simp: add.commute nat_mult_max_right)
+  ultimately have "2 ^ y * max (Max (range s2)) (max_const c2) < 2 ^ n"
+    by simp
+  moreover have "finite (range s2)" using finite_range_stays_finite Seq
+    by simp
+  ultimately show ?case using Seq \<open>2 ^ x * max (Max (range s1)) (max_const c1) < 2 ^ n\<close>
+    apply (subst IMP_To_IMP_Minus.simps)
+    apply(rule seq_terminates_when[where ?t1.0="100 * n * (x - Suc 0) + 50" and
+          ?t2.0="100 * n * (y - Suc 0) + 50"])
+      apply (drule bigstep_progress[where p = x] bigstep_progress[where p = y])+
+      apply(cases x)
+       apply simp_all
+    apply(cases y)
+    by (auto simp: algebra_simps)
+next
+  case (IfTrue s b c1 x t y c2)
+  hence "(2 ^ y) * Max (range s) < 2 ^ n"
+    by (meson le_less_trans max.cobounded1 move_exponent_to_rhs power_of_two_minus)
+  hence "Max (range s) < 2 ^ n" by(auto intro: le_less_trans[OF _ \<open>2 ^ y * Max (range s) < 2 ^ n\<close>])
+
+  with IfTrue show ?case apply auto
+    using local.IfTrue.hyps(1) apply auto
+  apply(simp only: t_small_step_fun_terminate_iff)
+    using IfTrue apply(simp add: t_small_step_fun_small_step_fun)
+    apply(rule t_small_step_fun_increase_time[where ?t="100 * n * (x - 1) + 50"])
+     apply(cases x)
+      using bigstep_progress IfTrue.IH bigstep_progress
+      by(fastforce simp: nat_mult_max_right)+
+next
+  case (IfFalse s b c2 x t y c1)
+  hence "(2 ^ y) * Max (range s) < 2 ^ n"
+    by (meson le_less_trans max.cobounded1 move_exponent_to_rhs power_of_two_minus)
+  hence "Max (range s) < 2 ^ n" by(auto intro: le_less_trans[OF _ \<open>2 ^ y * Max (range s) < 2 ^ n\<close>])
+  then show ?case
+    apply(subst t_small_step_fun_terminate_iff)
+    using IfFalse
+    using t_small_step_fun_small_step_fun
+    apply simp
+    apply(rule t_small_step_fun_increase_time[where ?t="100 * n * (x - 1) + 50"])
+     apply(cases x)
+    using bigstep_progress IfFalse.IH bigstep_progress
+    by(fastforce simp: nat_mult_max_right)+
+next
+  case (WhileFalse s b c)
+  hence "(2 ^ Suc (Suc 0)) * Max (range s) < 2 ^ n"
+    by (meson le_less_trans max.cobounded1 move_exponent_to_rhs power_of_two_minus)
+  hence "Max (range s) < 2 ^ n"
+    by(auto intro: le_less_trans[OF _ \<open>(2 ^ Suc (Suc 0)) * Max (range s) < 2 ^ n\<close>])
+  then show ?case using WhileFalse
+    by(simp add: t_small_step_fun_terminate_iff)
+next
+  case (WhileTrue s1 b c x s2 y s3 z)
+  hence "(2 ^ z) * Max (range s1) < 2 ^ n"
+    by (meson le_less_trans max.cobounded1 move_exponent_to_rhs power_of_two_minus)
+  hence "Max (range s1) < 2 ^ n" by(auto intro: le_less_trans[OF _ \<open>2 ^ z * Max (range s1) < 2 ^ n\<close>])
+  have "(2 :: nat) ^ x \<le> 2 ^ z" using WhileTrue by simp
+  hence "((2 :: nat) ^ x) * max (Max (range s1)) (max_const (WHILE b\<noteq>0 DO c)) < 2 ^ n"
+    using \<open>2 ^ z * max (Max (range s1)) (max_const (WHILE b\<noteq>0 DO c)) < 2 ^ n\<close>
+    by (meson leD leI less_le_trans mult_less_cancel2)
+  hence "2 ^ x * max (Max (range s1)) (max_const c) < 2 ^ n" by (simp add: nat_mult_max_right)
+  have "max (Max (range s1)) (max_const c) < 2 ^ (n - z)"
+    using power_of_two_minus WhileTrue by (metis max_const_com.simps)
+  have "Max (range s2) < 2 ^ (n - (y + 1))"
+    using IMP_space_growth[OF \<open>(c, s1) \<Rightarrow>\<^bsup> x \<^esup> s2\<close> \<open>finite (range s1)\<close>
+        \<open>max (Max (range s1)) (max_const c) < 2 ^ (n - z)\<close>] \<open>1 + x + y = z\<close> \<open>n > z \<close> by auto
+  hence "2 ^ (y + 1) * Max (range s2) < 2 ^ n" using move_exponent_to_rhs by blast
+  moreover have "2 ^ (y + 1) * max_const  (WHILE b\<noteq>0 DO c) < 2 ^ n"
+    using \<open>1 + x + y = z\<close> \<open>2 ^ z * max (Max (range s1)) (max_const (WHILE b\<noteq>0 DO c)) < 2 ^ n\<close>
+      power_of_two_increase_exponent_le[where ?a="1 + y" and ?b=x]
+    by(auto simp: add.commute nat_mult_max_right)
+  ultimately have "2 ^ (y + 1) * max (Max (range s2)) (max_const (WHILE b\<noteq>0 DO c)) < 2 ^ n"
+    by simp
+  moreover have "finite (range s2)" using finite_range_stays_finite WhileTrue by simp
+  ultimately show ?case using Seq \<open>2 ^ x * max (Max (range s1)) (max_const c) < 2 ^ n\<close>
+    apply(simp only: t_small_step_fun_terminate_iff)
+    using \<open>s1 b \<noteq> 0\<close> \<open>finite (range s1)\<close> \<open>Max (range s1) < 2 ^ n\<close>
+    apply(simp add:)
+    apply(rule seq_terminates_when[where ?t1.0="100 * n * (x - Suc 0) + 50" and
+          ?t2.0="100 * n * (y - Suc 0) + 50"])
+      using WhileTrue
+    using bigstep_progress by(auto simp: algebra_simps)
+qed auto
+
+text \<open>The other direction. Observe that we assume that the IMP program terminates after a limited
+      number of steps, that is, we don't show that termination of the IMP program follows from
+      termination of the translated IMP- program \<close>
+
+lemma IMP_Minus_To_IMP_aux:
+  assumes "(c :: IMP_com, s1) \<Rightarrow>\<^bsup>t'\<^esup> s2"
+    "t' \<le> t"
+    "finite (range s1)"
+    "n > t"
+    "((2 :: nat) ^ t) * (max (Max (range s1)) (max_const c)) < 2 ^ n"
+    "t_small_step_fun t''
+      (IMP_To_IMP_Minus c n, IMP_State_To_IMP_Minus s1 n)
+     = (SKIP, s2')"
+  shows
+    "s2' = IMP_State_To_IMP_Minus s2 n"
+proof -
+  have "t_small_step_fun (100 * n * (t' - 1) + 50)
+      (IMP_To_IMP_Minus c n, IMP_State_To_IMP_Minus s1 n)
+     = (SKIP, IMP_State_To_IMP_Minus s2 n)"
+    using assms by(fastforce intro: IMP_To_IMP_Minus dual_order.strict_trans2)
+  thus ?thesis by(metis Pair_inject assms less_imp_le_nat not_less t_small_step_fun_increase_time)
+qed
+
+subsection \<open>Variables\<close>
+
+text \<open>We give a few lemmas that specify what variables appear in translated IMP- programs. \<close>
+
+lemma IMP_To_IMP_Minus_variables:
+  "n > 0 \<Longrightarrow> set (enumerate_variables (IMP_To_IMP_Minus c n)) \<subseteq>
+    { var_bit_to_var (w, i) | w i. i \<le> n \<and> w \<in> set (vars c) }
+    \<union> { operand_bit_to_var (op, i) | op i. i < n \<and> (op = a_chr \<or> op = b_chr) }
+    \<union> { carry, zero }"
+proof(induction c)
+  case SKIP
+  then show ?case by(auto simp: enumerate_variables_def)
+next
+  case (Assign v a)
+  thus ?case using assignment_to_binary_variables[where ?n=n and ?v=v and ?a=a] by auto
+next
+  case (Seq c1 c2)
+  then show ?case by(auto simp: set_enumerate_variables_seq)
+next
+  case (If x1 c1 c2)
+  then show ?case by (auto simp: set_enumerate_variables_if)
+next
+  case (While x1 c)
+  then show ?case by (auto simp: set_enumerate_variables_while)
+qed
+
+lemma card_of_set_comprehension_of_set_list: "card { f x |x. x \<in> set l} \<le> length (remdups l)"
+proof(induction l)
+  case (Cons a l)
+  have "{ f x |x. x \<in> set (a # l)} = { f a } \<union> { f x |x. x \<in> set l}" by auto
+  thus ?case using Cons apply auto
+     apply (metis (mono_tags, lifting) card.infinite card_insert_if finite_insert mem_Collect_eq)
+    by (metis (no_types, lifting) Suc_le_mono card.infinite card_insert_disjoint finite_insert
+        insert_absorb le_SucI)
+qed auto
+
+lemma card_union_le: "card U \<le> a \<Longrightarrow> card W \<le> b \<Longrightarrow> card (U \<union> W) \<le> (a + b)"
+  using card_Un_le[where ?A=U and ?B=W] by simp
+
+lemma card_union_le_intro: "card U \<le> a \<Longrightarrow> card W \<le> b \<Longrightarrow> c \<ge> a + b \<Longrightarrow> card (U \<union> W) \<le> c"
+  using card_Un_le[where ?A=U and ?B=W] by simp
+
+lemma IMP_To_IMP_Minus_variables_length:
+  assumes "n > 0"
+  shows "length (enumerate_variables (IMP_To_IMP_Minus c n)) \<le>
+    (n + 2) * (num_vars c) + 2 * n + 2"
+proof -
+  have "card  { var_bit_to_var (w, i) | w i. i = n \<and> w \<in> set (vars c)} \<le> card (set (vars c))"
+    using card_of_set_comprehension_of_set_list length_remdups_card_conv by metis
+  moreover have "num_vars c = card (set (vars c))"
+    by (simp add: length_remdups_card_conv num_vars_def)
+  ultimately have "card  { var_bit_to_var (w, i) | w i. i = n \<and> w \<in> set (vars c)} \<le> num_vars c"
+    by linarith
+
+  moreover have "finite { var_bit_to_var (w, i) | w i. i < n \<and> w \<in> set (vars c) }
+    \<and> card { var_bit_to_var (w, i) | w i. i < n \<and> w \<in> set (vars c) }
+    \<le> n * (num_vars c)"
+  proof(induction n)
+    case (Suc n)
+    have "{var_bit_to_var (w, i) |w i. i < Suc n \<and> w \<in> set (vars c)}
+      = {var_bit_to_var (w, i) |w i. i < n \<and> w \<in> set (vars c)}
+        \<union> { var_bit_to_var (w, n) |w. w \<in> set (vars c) }"
+      by auto
+    moreover have "card {var_bit_to_var (w, n) |w. w \<in> set (vars c)}
+      \<le> num_vars c"
+      using card_of_set_comprehension_of_set_list num_vars_def by fastforce
+    ultimately show ?case using Suc by (simp add: card_union_le sup_commute)
+  qed auto
+
+  moreover have *: "{ var_bit_to_var (w, i) | w i. i \<le> n \<and> w \<in> set (vars c) } =
+  { var_bit_to_var (w, i) | w i. i < n \<and> w \<in> set (vars c) } \<union> { var_bit_to_var (w, i) | w i. i = n \<and> w \<in> set (vars c)}"
+    by auto
+  ultimately have "finite { var_bit_to_var (w, i) | w i. i \<le> n \<and> w \<in> set (vars c) }
+    \<and> card { var_bit_to_var (w, i) | w i. i \<le> n \<and> w \<in> set (vars c) }
+    \<le> n * (num_vars c) + num_vars c"
+    by (subst *) (auto simp: card_union_le)
+
+  moreover have "card {CHR ''?'' # sep2 # w |w. w \<in> set (vars c)}
+    \<le> num_vars c" using card_of_set_comprehension_of_set_list num_vars_def by fastforce
+  moreover have "finite {operand_bit_to_var (op, i) |op i. i < n \<and> (op = a_chr \<or> op = b_chr)}
+    \<and> card { operand_bit_to_var (op, i) |op i. i < n \<and> (op = a_chr \<or> op = b_chr) } \<le> 2 * n"
+  proof (induction n)
+    case (Suc n)
+    have "{operand_bit_to_var (op, i) |op i. i < Suc n \<and> (op = a_chr \<or> op = b_chr)}
+      = { operand_bit_to_var (op, i) |op i. i < n \<and> (op = a_chr \<or> op = b_chr) }
+        \<union> { operand_bit_to_var (a_chr, n), operand_bit_to_var (b_chr, n)}" by auto
+    thus ?case using Suc by(auto intro!: card_insert_le_m1)
+  qed auto
+  ultimately have
+    f: "finite ({ var_bit_to_var (w, i) | w i. i \<le> n \<and> w \<in> set (vars c) }
+    \<union> { operand_bit_to_var (op, i) | op i. i < n \<and> (op = a_chr \<or> op = b_chr) }
+    \<union> { carry, zero })" and
+    "card ({ var_bit_to_var (w, i) | w i. i \<le> n \<and> w \<in> set (vars c) }
+    \<union> { operand_bit_to_var (op, i) | op i. i < n \<and> (op = a_chr \<or> op = b_chr) }
+    \<union> { carry, zero }) \<le> (n + 1) * (num_vars c) + 2 * n + 2"
+    by(auto simp: card_union_le intro!: card_insert_le_m1 card_union_le_intro)
+  hence "card (set (enumerate_variables (IMP_To_IMP_Minus c n)))
+    \<le> (n + 2) * (num_vars c) + 2 * n + 2"
+    using card_mono[OF f IMP_To_IMP_Minus_variables[OF \<open>n > 0\<close>]] by simp
+  thus ?thesis by(simp add:  distinct_card[OF enumerate_variables_distinct])
+qed
+
+lemma var_bit_in_IMP_Minus_variables_then_bit_less_n: "n > 0 \<Longrightarrow> var_bit_to_var (a, Suc b)
+           \<in> set (enumerate_variables (IMP_To_IMP_Minus c n)) \<Longrightarrow> b \<le> n"
+  apply(frule set_mp[OF IMP_To_IMP_Minus_variables])
+  by auto
+
+lemma var_bit_in_IMP_Minus_variables: "
+v \<in> set (vars c) \<Longrightarrow> 
+  (\<forall>i < n. var_bit_to_var (v, Suc i) \<in> set (enumerate_variables (IMP_To_IMP_Minus c n))) \<or> 
+  var_bit_to_var (v,0) \<in> set (enumerate_variables (IMP_To_IMP_Minus c n))"
+  apply(induction c)
+  by(auto simp: assignment_to_binary_def binary_adder_def set_enumerate_variables_seq
+      copy_atom_to_operand_variables adder_def com_list_to_seq_variables full_adder_variables
+      binary_subtractor_def subtract_handle_underflow_variables set_enumerate_variables_if
+      set_enumerate_variables_while split: aexp.splits atomExp.splits)
+
+end
